axioms.bpl
@@ -21,6 +21,14 @@ function target__load_64(Tr, bv64) returns (bv64);
 function target__trace_load_64(Tr, bv64) returns (Tr);
 function target__store_64(Tr, bv64, bv64) returns (Tr);
 
+
+function source__trace_load_128(Tr, bv64) returns (Tr);
+function source__load_128(Tr, bv64) returns (bv128);
+function source__store_128(Tr, bv64, bv128) returns (Tr);
+function target__load_128(Tr, bv64) returns (bv128);
+function target__trace_load_128(Tr, bv64) returns (Tr);
+function target__store_128(Tr, bv64, bv128) returns (Tr);
+
 axiom (forall source__tr: Tr, target__tr: Tr, source__addr: bv64, target__addr: bv64, source__value: bv8, target__value: bv8 :: 
         {source__store_8(source__tr,source__addr,source__value), target__store_8(target__tr,target__addr,target__value)}
         (source__tr == target__tr && source__addr == target__addr && source__value == target__value) ==> 
@@ -33,7 +41,6 @@ axiom (forall source__tr: Tr, target__tr: Tr, source__addr: bv64, target__addr: 
 axiom (forall source__tr: Tr, target__tr: Tr, source__addr: bv64, target__addr: bv64 :: 
         {source__trace_load_8(source__tr,source__addr), target__trace_load_8(target__tr,target__addr)}
         (source__tr == target__tr && source__addr == target__addr) ==> (source__trace_load_8(source__tr,source__addr) == target__trace_load_8(target__tr,target__addr)));
-
 
 
 axiom (forall source__tr: Tr, target__tr: Tr, source__addr: bv64, target__addr: bv64, source__value: bv32, target__value: bv32 :: 
@@ -62,3 +69,21 @@ axiom (forall source__tr: Tr, target__tr: Tr, source__addr: bv64, target__addr: 
 axiom (forall source__tr: Tr, target__tr: Tr, source__addr: bv64, target__addr: bv64 :: 
         {source__trace_load_64(source__tr,source__addr), target__trace_load_64(target__tr,target__addr)}
         (source__tr == target__tr && source__addr == target__addr) ==> (source__trace_load_64(source__tr,source__addr) == target__trace_load_64(target__tr,target__addr)));
+
+
+
+
+axiom (forall source__tr: Tr, target__tr: Tr, source__addr: bv64, target__addr: bv64, source__value: bv128, target__value: bv128 :: 
+        {source__store_128(source__tr,source__addr,source__value), target__store_128(target__tr,target__addr,target__value)}
+        (source__tr == target__tr && source__addr == target__addr && source__value == target__value) ==> 
+        (source__store_128(source__tr,source__addr,source__value) == target__store_128(target__tr,target__addr,target__value)));
+
+axiom (forall source__tr: Tr, target__tr: Tr, source__addr: bv64, target__addr: bv64 :: 
+        {source__load_128(source__tr,source__addr), target__load_128(target__tr,target__addr)}
+        (source__tr == target__tr && source__addr == target__addr) ==> (source__load_128(source__tr,source__addr) == target__load_128(target__tr,target__addr)));
+
+axiom (forall source__tr: Tr, target__tr: Tr, source__addr: bv64, target__addr: bv64 :: 
+        {source__trace_load_128(source__tr,source__addr), target__trace_load_128(target__tr,target__addr)}
+        (source__tr == target__tr && source__addr == target__addr) ==> (source__trace_load_128(source__tr,source__addr) == target__trace_load_128(target__tr,target__addr)));
+
+
